src/Helpers/RelationTheorems.v
@@ -3,6 +3,7 @@ Require Import Helpers.RelationRewriting.
 
 Import RelationNotations.
 
+(*
 Theorem seq_star_invariant A (r: relation A A unit) P :
   (test P;; r) ---> (test P;; r;; test P) ->
   (test P;; seq_star r) ---> (test P;; seq_star r;; test P).
@@ -18,6 +19,7 @@ Proof.
   - setoid_rewrite <- seq_star1 at 2; norm.
     setoid_rewrite test_to_id at 2; norm.
 Qed.
+*)
 
 Fixpoint seq_rep_n {A T} (n: nat) (p: relation A A T) : relation A A T :=
   match n with
@@ -31,43 +33,47 @@ Fixpoint bind_rep_n {A T} (n: nat) (p: T -> relation A A T) (o: T) : relation A 
   | S n' => x <- p o; bind_rep_n n' p x
   end.
 
-Lemma seq_star_inv_rep_n A T (p: relation A A T) a1 a2 t:
-  seq_star p a1 a2 t ->
-  exists n, seq_rep_n n p a1 a2 t.
+Fixpoint bind_rep_r_n {A T} (n: nat) (p: T -> relation A A T) (o: T) : relation A A T :=
+  match n with
+  | O => pure o
+  | S n' => x <- bind_rep_r_n n' p o; p x
+  end.
+
+Lemma seq_star_inv_rep_n A T (p: relation A A T) a1 a2:
+  seq_star p a1 a2 ->
+  exists n, seq_rep_n n p a1 a2.
+Proof.
+  induction 1.
+  - exists O. do 2 econstructor.
+  - destruct IHseq_star as (n&?). exists (S n). destruct_return.
+    * simpl. econstructor. do 2 eexists; intuition eauto.
+    * simpl. right. do 2 eexists; intuition eauto.
+  - exists 1. econstructor; eauto.
+Qed.
+
+Lemma bind_star_inv_rep_n A T (p: T -> relation A A T) (o: T) a1 a2:
+  bind_star p o a1 a2 ->
+  exists n, bind_rep_n n p o a1 a2.
 Proof.
   induction 1.
   - exists O; firstorder.
-  - destruct IHseq_star as (n&?). exists (S n).
-    simpl. do 2 eexists; intuition eauto.
+  - destruct IHbind_star as (n&?). exists (S n). destruct_return.
+    * simpl. do 2 eexists; intuition eauto.
+    * simpl. right. do 2 eexists; intuition eauto.
+  - exists 1. econstructor; eauto.
 Qed.
 
-Lemma bind_star_inv_rep_n A T (p: T -> relation A A T) (o: T) a1 a2 t:
-  bind_star p o a1 a2 t ->
-  exists n, bind_rep_n n p o a1 a2 t.
+Lemma bind_star_rep_n_to_bind_star A T (p: T -> relation A A T) (o: T) a1 a2 n:
+  bind_rep_n n p o a1 a2 ->
+  bind_star p o a1 a2.
 Proof.
-  induction 1.
-  - exists O; firstorder.
-  - destruct IHbind_star as (n&?). exists (S n).
-    simpl. do 2 eexists; intuition eauto.
-Qed.
-
-Lemma bind_star_rep_n_to_bind_star A T (p: T -> relation A A T) (o: T) a1 a2 t n:
-  bind_rep_n n p o a1 a2 t ->
-  bind_star p o a1 a2 t.
-Proof.
-  revert o a1 a2 t. induction n; intros o a1 a2 t.
+  revert o a1 a2. induction n; intros o a1 a2.
   - simpl. inversion 1; subst. apply bind_star_pure.
-  - simpl. intros (v&a'&?&?).
-    econstructor; eauto.
-Qed.
-
-Lemma bind_star_trans A T (p: T -> relation A A T) (o1 o2 o3: T) (a1 a2 a3: A):
-  bind_star p o1 a1 a2 o2 ->
-  bind_star p o2 a2 a3 o3 ->
-  bind_star p o1 a1 a3 o3.
-Proof.
-  intros Hleft. revert o3 a3. induction Hleft; intros ??; auto.
-  intros. econstructor; eauto.
+  - simpl. destruct_return.
+    * intros (v&a'&?&?). econstructor; eauto.
+    * intros [?|(?&?&?&?)].
+      ** eapply bind_star_one_more_err; eauto.
+      ** eapply bind_star_one_more_valid; eauto 10.
 Qed.
 
 Lemma seq_star_rep_n_ind {A1 A2 T1 T2} (p: relation A1 A2 T1) q (r: relation A1 A2 T2):
@@ -75,25 +81,86 @@ Lemma seq_star_rep_n_ind {A1 A2 T1 T2} (p: relation A1 A2 T1) q (r: relation A1 
   (p ;; seq_star q) ---> r.
 Proof.
   intros.
-  intros a1 a2 t2 Hl.
-  destruct Hl as (t1&a2'&Hp&Hstar).
-  eapply seq_star_inv_rep_n in Hstar as (n&?).
-  eapply H; do 2 eexists; intuition eauto.
+  intros a1 a2 Hl.
+  destruct_return.
+  * destruct Hl as (t1&a2'&Hp&Hstar).
+    eapply seq_star_inv_rep_n in Hstar as (n&?).
+    eapply H; do 2 eexists; intuition eauto.
+  * destruct Hl as [Hhd|(?&?&Hp&Hstar)].
+    ** eapply (H O). left; eauto.
+    ** eapply seq_star_inv_rep_n in Hstar as (n&?).
+       eapply H. right. eauto.
 Qed.
 
-Lemma seq_star_alt A T r (x y: A) (t: T):
-  seq_star r x y t <-> (exists n, seq_rep_n n r x y t).
+Lemma bind_star_rep_n_ind {A1 A2 T1} (p: relation A1 A2 T1) q (r: relation A1 A2 T1):
+  (forall n, (o <- p; bind_rep_n n q o) ---> r) ->
+  (o <- p; bind_star q o) ---> r.
+Proof.
+  intros.
+  intros a1 a2 Hl.
+  destruct_return.
+  * destruct Hl as (t1&a2'&Hp&Hstar).
+    eapply bind_star_inv_rep_n in Hstar as (n&?).
+    eapply H; do 2 eexists; intuition eauto.
+  * destruct Hl as [Hhd|(?&?&Hp&Hstar)].
+    ** eapply (H O). left; eauto.
+    ** eapply bind_star_inv_rep_n in Hstar as (n&?).
+       eapply H. right. eauto.
+Qed.
+
+Lemma seq_star_alt A T r (x : A) (y: Return A T):
+  seq_star r x y <-> (exists n, seq_rep_n n r x y).
 Proof.
   split.
   - induction 1.
-    * exists O. econstructor.
+    * exists O. econstructor; eauto.
     * destruct IHseq_star as (n&Hseq).
-      exists (S n). econstructor; eauto.
+      exists (S n). destruct_return.
+      ** econstructor; eauto.
+      ** right. eauto 10.
+    * exists (S O). econstructor; eauto.
   - intros (n&Hseq). revert x y Hseq.
     induction n; intros x y Hseq.
     * inversion Hseq; subst; econstructor.
-    * destruct Hseq as (t'&?&?&?).
-      econstructor; eauto.
+    * destruct_return.
+      ** destruct Hseq as (t'&?&?&?).
+         econstructor; eauto.
+      ** destruct Hseq as [Hhd|(?&?&?&?)].
+         *** eapply seq_star_one_more_err; eauto.
+         *** eapply seq_star_one_more_valid; eauto.
+Qed.
+
+Lemma bind_rep_lr_n A T (r: T -> relation A A T) o n:
+  bind_rep_n n r o <---> bind_rep_r_n n r o.
+Proof.
+  revert o. induction n; intros o.
+  { reflexivity. }
+  simpl. setoid_rewrite IHn. clear.
+  induction n.
+  - simpl. rew bind_right_id.
+  - simpl. rew<- IHn.
+Qed.
+
+Lemma bind_star_alt A T r (x : A) o (y: Return A T):
+  bind_star r o x y <-> (exists n, bind_rep_n n r o x y).
+Proof.
+  split.
+  - induction 1.
+    * exists O. econstructor; eauto.
+    * destruct IHbind_star as (n&Hseq).
+      exists (S n). destruct_return.
+      ** econstructor; eauto.
+      ** right. eauto 10.
+    * exists (S O). econstructor; eauto.
+  - intros (n&Hseq). revert o x y Hseq.
+    induction n; intros o x y Hseq.
+    * inversion Hseq; subst; econstructor.
+    * destruct_return.
+      ** destruct Hseq as (t'&?&?&?).
+         eapply bind_star_one_more_valid; eauto.
+      ** destruct Hseq as [Hhd|(?&?&?&?)].
+         *** eapply bind_star_one_more_err; eauto.
+         *** eapply bind_star_one_more_valid; eauto.
 Qed.
 
 Lemma seq_star_mid_invariant A (p: relation A A unit) (q: relation A A unit) P:
@@ -130,3 +197,90 @@ Proof.
   - setoid_rewrite IHn.
     apply any_idem.
 Qed.
+
+Theorem bind_star_ind_r A B T1 (q x: relation A B T1) (p: T1 -> relation B B T1) :
+  q + and_then x p ---> x ->
+  and_then q (bind_star p) ---> x.
+Proof.
+  intros Himpl.
+  assert (q ---> x) as ->.
+  { rew<- Himpl. Left. }
+  assert (and_then x p ---> x) as Himpl'.
+  { setoid_rewrite <-Himpl at 2. Right. }
+  eapply bind_star_rep_n_ind. intros n.
+  induction n.
+  - simpl. rew bind_right_id.
+  - simpl. setoid_rewrite <-bind_assoc. rew Himpl'. eauto.
+Qed.
+
+Theorem bind_star_ind_r_pure A T1 t (x: relation A A T1) (p: T1 -> relation A A T1):
+  (pure t) + and_then x p ---> x ->
+  bind_star p t ---> x.
+Proof.
+  specialize (@bind_star_ind_r A A _ (pure t) x p).
+  setoid_rewrite bind_left_id; auto.
+Qed.
+
+Theorem simulation_seq A B
+        (p: relation A B unit)
+        (q: relation B B unit)
+        (r: relation A A unit) :
+  (p;; q) ---> (r;; p) ->
+  (p;; seq_star q) ---> (seq_star r;; p).
+Proof.
+  intros Hconv.
+  apply seq_star_rep_n_ind. intros n.
+
+  induction n. simpl.
+  - setoid_rewrite <-seq_star_none.
+    rew unit_identity.
+    rew bind_right_id_unit.
+  - simpl.
+    setoid_rewrite <-bind_assoc.
+    rew Hconv. rew IHn.
+    setoid_rewrite <-bind_assoc.
+    setoid_rewrite seq_star_fold; reflexivity.
+Qed.
+
+Theorem simulation_seq_value A B T
+        (p: relation A B unit)
+        (q: relation B B T)
+        (r: relation A A T) :
+  (p;; q) ---> (v <- r; (p;; pure v)) ->
+  (p;; seq_star q) ---> (v <- seq_star r; (p;; pure v)).
+Proof.
+Admitted.
+(*
+  intros Hconv.
+  apply seq_star_rep_n_ind. intros n.
+
+  induction n. simpl.
+  - setoid_rewrite <-seq_star_none.
+    rew unit_identity.
+    rew bind_right_id_unit.
+  - simpl.
+    setoid_rewrite <-bind_assoc.
+    rew Hconv. rew IHn.
+    setoid_rewrite <-bind_assoc.
+    setoid_rewrite seq_star_fold; reflexivity.
+  setoid_rewrite seq_star_lr.
+  t.
+  induction H1; propositional.
+  - eauto 15.
+  - repeat match goal with
+           | [ u: unit |- _ ] => destruct u
+           end.
+    unfold rimpl in H; simpl in *.
+    specialize (H y0 z o2).
+    match type of H with
+    | ?P -> ?Q =>
+      let HP := fresh in
+      assert P as HP;
+        [ | specialize (H HP) ]
+    end; eauto; propositional.
+    eauto 15.
+
+    Grab Existential Variables.
+    all: auto.
+Qed.
+*)
